Update most interop stubs + Clean up .vaf

vale/code/arch/x64/interop/Main.ml
@@ -26,85 +26,111 @@ let aes_encrypt_block = ("AESEncryptBlockStdcall", [
   Modifies ["output_b"],
   Return Unit)
 
+let aes_encrypt_block_be = ("aes_EncryptBlockBEStdcall", [
+  ("output_b", TBuffer TUInt128, Sec); ("input_b", TBuffer TUInt128, Sec);
+  ("key", TGhost "aes_key_LE AES_128", Pub); ("keys_b", TBuffer TUInt128, Sec)
+  ], 
+  SaveRegsStk true,
+  AddStk (Prims.parse_int "0"),
+  Modifies ["output_b"],
+  Return Unit
+  )
 
-(*
-let ghash = ("ghash_incremental_bytes_stdcall_win", [
+let ghash = ("ghash_incremental_bytes_stdcall", [
   ("h_b", TBuffer TUInt128, Sec); ("hash_b", TBuffer TUInt128, Sec);
   ("input_b", TBuffer TUInt128, Sec); ("num_bytes", TBase TUInt64, Pub)
-  ], Stk (Prims.parse_int "5"))
-*)
+  ], 
+  SaveRegsStk true,
+  AddStk (Prims.parse_int "0"),
+  Modifies ["hash_b"],
+  Return Unit)
 
-(*
-let gctr_bytes_extra_buffer = ("gctr_bytes_extra_buffer_win", [
-  ("plain_b", TBuffer TUInt128, Sec); ("num_bytes", TBase TUInt64, Pub);
-  ("iv_old", TGhost "quad32", Pub); ("iv_b", TBuffer TUInt128, Sec);
-  ("key", TGhost "aes_key_LE AES_128", Pub); ("keys_b", TBuffer TUInt128, Sec);
-  ("cipher_b", TBuffer TUInt128, Sec)], Stk (Prims.parse_int "0"))
-*)
-
-(*
-let ghash_extra = ("ghash_incremental_extra_stdcall_win", [
+let ghash_extra = ("ghash_extra_stdcall", [
   ("in_b", TBuffer TUInt128, Sec); ("hash_b", TBuffer TUInt128, Sec);
   ("h_b", TBuffer TUInt128, Sec); ("num_bytes", TBase TUInt64, Pub);
-  ("orig_hash", TGhost "quad32", Pub)], Stk (Prims.parse_int "4"))
-*)
+  ("orig_hash", TGhost "quad32", Pub)], 
+  SaveRegsStk true,
+  AddStk (Prims.parse_int "0"),
+  Modifies ["hash_b"],
+  Return Unit)
 
-(*
-let ghash_one_block = ("ghash_incremental_one_block_buffer_win", [
+let ghash_one_block = ("ghash_one_block", [
   ("h_b", TBuffer TUInt128, Sec); ("hash_b", TBuffer TUInt128, Sec);
   ("input_b", TBuffer TUInt128, Sec); ("offset", TBase TUInt64, Pub)
-  ], Stk (Prims.parse_int "4"))
-*)
+  ], 
+  SaveRegsStk true,
+  AddStk (Prims.parse_int "0"),
+  Modifies ["hash_b"],
+  Return Unit)
 
-(*
-let inc32 = ("inc32_buffer_win", [("iv_b", TBuffer TUInt128, Sec)], Stk (Prims.parse_int "0"))
-*)
-
- (*
-let quad32_xor = ("quad32_xor_buffer", [("src1", TBuffer TUInt128, Sec);
-  ("src2", TBuffer TUInt128, Sec); ("dst", TBuffer TUInt128, Sec)], Stk (Prims.parse_int "0"))
-*)
-
-(*
-let gcm_make_length = ("gcm_make_length_quad_buffer_win", [
-  ("plain_num_bytes", TBase TUInt64, Pub); ("auth_num_bytes", TBase TUInt64, Pub);
-  ("b", TBuffer TUInt128, Sec)], Stk (Prims.parse_int "0"))
-*)
-
-(*
-let gcm_load_xor = ("gcm_load_xor_store_buffer_win", [
+let gcm_load_xor = ("gcm_load_xor_stdcall", [
   ("plain_b", TBuffer TUInt128, Sec); ("mask_b", TBuffer TUInt128, Sec);
   ("cipher_b", TBuffer TUInt128, Sec); ("offset", TBase TUInt64, Sec);
   ("num_blocks", TGhost "nat64", Pub);
-  ("key", TGhost "aes_key_LE AES_128", Pub); ("iv", TGhost "quad32", Pub)], Stk (Prims.parse_int "0"))
-*)
+  ("key", TGhost "aes_key_LE AES_128", Pub); ("iv", TGhost "quad32", Pub)], 
+  SaveRegsStk false,
+  AddStk (Prims.parse_int "0"),
+  Modifies ["cipher_b"],
+  Return Unit)
 
-(*
-let aes_encrypt_block_be = ("aes128_encrypt_block_be_win", [
-  ("output_b", TBuffer TUInt128, Sec); ("input_b", TBuffer TUInt128, Sec);
-  ("key", TGhost "aes_key_LE AES_128", Pub); ("keys_b", TBuffer TUInt128, Sec)
-  ], Stk (Prims.parse_int "0"))
-*)
+let inc32 = ("inc32_stdcall", [("iv_b", TBuffer TUInt128, Sec)], 
+  SaveRegsStk false,
+  AddStk (Prims.parse_int "0"),
+  Modifies ["iv_b"],
+  Return Unit)
 
-(*
-let mk_quad1 = ("mk_quad32_lo0_be_1_buffer_win", [("b", TBuffer TUInt128, Sec)], Stk (Prims.parse_int "0"))
-*)
-(*
-let zero_quad32_buffer = ("zero_quad32_buffer_win", [("b", TBuffer TUInt128, Sec)], Stk (Prims.parse_int "0"))
-*)
-(*
-let reverse_quad32 = ("reverse_bytes_quad32_buffer_win", [("b", TBuffer TUInt128, Sec)], Stk (Prims.parse_int "0"))
-*)
+let zero_quad32 = ("zero_quad32_stdcall", [("b", TBuffer TUInt128, Sec)],
+  SaveRegsStk false,
+  AddStk (Prims.parse_int "0"),
+  Modifies ["b"],
+  Return Unit)
 
-(*
+let reverse_quad32 = ("reverse_quad32_stdcall", [("b", TBuffer TUInt128, Sec)], 
+  SaveRegsStk false,
+  AddStk (Prims.parse_int "0"),
+  Modifies ["b"],
+  Return Unit)
+
+let mk_quad1 = ("mk_quad32_lo0_be_1_stdcall", [("b", TBuffer TUInt128, Sec)], 
+  SaveRegsStk false,
+  AddStk (Prims.parse_int "0"),
+  Modifies ["b"],
+  Return Unit)
+
+let gcm_make_length = ("gcm_make_length_stdcall", [
+  ("plain_num_bytes", TBase TUInt64, Pub); ("auth_num_bytes", TBase TUInt64, Pub);
+  ("b", TBuffer TUInt128, Sec)], 
+  SaveRegsStk false,
+  AddStk (Prims.parse_int "0"),
+  Modifies ["b"],
+  Return Unit)
+
+let gctr_bytes_extra = ("gctr_bytes_extra_stdcall", [
+  ("plain_b", TBuffer TUInt128, Sec); ("num_bytes", TBase TUInt64, Pub);
+  ("iv_old", TGhost "quad32", Pub); ("iv_b", TBuffer TUInt128, Sec);
+  ("key", TGhost "aes_key_LE AES_128", Pub); ("keys_b", TBuffer TUInt128, Sec);
+  ("cipher_b", TBuffer TUInt128, Sec)], 
+  SaveRegsStk false,
+  AddStk (Prims.parse_int "0"),
+  Modifies ["cipher_b"],
+  Return Unit)
+
+
+let quad32_xor = ("quad32_xor_stdcall", [("src1", TBuffer TUInt128, Sec);
+  ("src2", TBuffer TUInt128, Sec); ("dst", TBuffer TUInt128, Sec)], 
+  SaveRegsStk false,
+  AddStk (Prims.parse_int "0"),
+  Modifies ["dst"],
+  Return Unit)
+
 let sha_update_bytes =
    ("sha_update_bytes_stdcall",  
   [("ctx_b", TBuffer TUInt128, Sec);  ("in_b", TBuffer TUInt128, Sec); 
     ("num_val", TBase TUInt64, Sec); ("k_b", TBuffer TUInt128, Sec)], 
   SaveRegsStk true,
   AddStk (Prims.parse_int "0"),
-  Modifies ["ctx_b"])
-*)
+  Modifies ["ctx_b"],
+  Return Unit)
 
 let memcpy = ("memcpy", [("dst", TBuffer TUInt64, Sec); ("src", TBuffer TUInt64, Sec)], SaveRegsStk false, AddStk (Prims.parse_int "0"), Modifies ["dst"], Return Unit)
 
@@ -123,7 +149,7 @@ let check_aesni = ("check_aesni_stdcall", [], SaveRegsStk false, AddStk (Prims.p
 
 let check_sha = ("check_sha_stdcall", [], SaveRegsStk false, AddStk (Prims.parse_int "0"), Modifies [], Return Int64)
 
-let name = aes_encrypt_block 
+let name = sha_update_bytes 
 
 let _ = print_string (translate_vale X86 name)
 let _ = print_newline()
