vale/code/arch/x64/interop/GHash_extra_stdcall.fsti
@@ -1,0 +1,89 @@
+module GHash_extra_stdcall
+
+open LowStar.Buffer
+module B = LowStar.Buffer
+module BV = LowStar.BufferView
+open LowStar.Modifies
+module M = LowStar.Modifies
+open LowStar.ModifiesPat
+open FStar.HyperStack.ST
+module HS = FStar.HyperStack
+open Interop
+open Words_s
+open Types_s
+open GCTR_s
+open GCTR
+open GCM_s
+open GCM_helpers
+open GHash
+open X64.CPU_Features_s
+
+let buffer_to_quad32 (b:s8 { B.length b % 16 == 0 /\ B.length b > 0 }) (h:HS.mem) : GTot quad32 =
+  let b128 = BV.mk_buffer_view b Views.view128 in
+  BV.as_buffer_mk_buffer_view b Views.view128;
+  BV.get_view_mk_buffer_view b Views.view128;
+  BV.length_eq b128;
+  assert (B.length b >= 16);
+  assert (BV.length b128 > 0);
+  BV.sel h b128 0
+
+let buffer_to_seq_quad32 (b:s8 { B.length b % 16 == 0 }) (h:HS.mem) : GTot (s:Seq.seq quad32 {Seq.length s == B.length b / 16} ) =
+  let b128 = BV.mk_buffer_view b Views.view128 in
+  BV.as_buffer_mk_buffer_view b Views.view128;
+  BV.get_view_mk_buffer_view b Views.view128;
+  BV.length_eq b128;
+  (BV.as_seq h b128)
+
+let pre_cond (h:HS.mem) (in_b:s8) (hash_b:s8) (h_b:s8) (num_bytes:UInt64.t) (orig_hash:Ghost.erased (quad32)) = 
+  pclmulqdq_enabled /\
+  live h in_b /\ live h hash_b /\ live h h_b /\  
+  disjoint in_b hash_b /\ 
+  disjoint in_b h_b /\ 
+  disjoint hash_b h_b /\ 
+  length in_b % 16 == 0 /\ length hash_b % 16 == 0 /\ length h_b % 16 == 0 /\
+  length in_b == bytes_to_quad_size (UInt64.v num_bytes) `op_Multiply` 16 /\
+  length h_b == 16 /\
+  length hash_b == 16 /\
+  4096 `op_Multiply` (UInt64.v num_bytes) < pow2_32 /\
+  256 `op_Multiply` bytes_to_quad_size (UInt64.v num_bytes) < pow2_32 /\
+
+  (let num_bytes = UInt64.v num_bytes in
+   let num_blocks = num_bytes / 16 in
+   let old_hash = buffer_to_quad32 hash_b h in
+   let h_val = buffer_to_quad32 h_b h in
+   // GHash reqs
+   let input = Seq.slice (buffer_to_seq_quad32 in_b h) 0 num_blocks in
+   old_hash == ghash_incremental0 h_val (Ghost.reveal orig_hash) input /\
+
+   // Extra reqs
+   num_bytes % 16 <> 0 /\
+   0 < num_bytes /\ num_bytes < 16 `op_Multiply` bytes_to_quad_size num_bytes /\
+   16 `op_Multiply` (bytes_to_quad_size num_bytes - 1) < num_bytes)
+
+let post_cond (h:HS.mem) (h':HS.mem) (in_b:s8) (hash_b:s8) (h_b:s8) (num_bytes:UInt64.t) (orig_hash:Ghost.erased (quad32)) = 
+  live h in_b /\ live h hash_b /\ live h h_b /\
+  live h' in_b /\ live h' hash_b /\ live h' h_b /\
+  length in_b % 16 == 0 /\ length hash_b % 16 == 0 /\ length h_b % 16 == 0 /\
+  length in_b  == bytes_to_quad_size (UInt64.v num_bytes) `op_Multiply` 16 /\
+  length h_b == 16 /\
+  length hash_b == 16 /\
+  (let num_bytes = UInt64.v num_bytes in
+   let num_blocks = num_bytes / 16 in
+   let old_hash = buffer_to_quad32 hash_b h in
+   let new_hash = buffer_to_quad32 hash_b h' in
+   let h_val = buffer_to_quad32 h_b h in
+
+   let input_bytes = Seq.slice (le_seq_quad32_to_bytes (buffer_to_seq_quad32 in_b h')) 0 num_bytes in
+   let padded_bytes = pad_to_128_bits input_bytes in
+   let input_quads = le_bytes_to_seq_quad32 padded_bytes in
+   (num_bytes > 0 ==> Seq.length input_quads > 0 /\
+                       new_hash == ghash_incremental h_val (Ghost.reveal orig_hash) input_quads)
+    )  
+
+let full_post_cond (h:HS.mem) (h':HS.mem) (in_b:s8) (hash_b:s8) (h_b:s8) (num_bytes:UInt64.t) (orig_hash:Ghost.erased (quad32))  =
+  post_cond h h' in_b hash_b h_b num_bytes orig_hash  /\
+  M.modifies (M.loc_buffer hash_b) h h'
+
+val ghash_extra_stdcall: in_b:s8 -> hash_b:s8 -> h_b:s8 -> num_bytes:UInt64.t -> orig_hash:Ghost.erased (quad32) -> Stack unit
+	(requires (fun h -> pre_cond h in_b hash_b h_b num_bytes orig_hash ))
+	(ensures (fun h0 _ h1 -> full_post_cond h0 h1 in_b hash_b h_b num_bytes orig_hash ))
