vale/code/arch/x64/interop/GHash_incremental_bytes_stdcall.fsti
@@ -1,0 +1,75 @@
+module GHash_incremental_bytes_stdcall
+
+open LowStar.Buffer
+module B = LowStar.Buffer
+module BV = LowStar.BufferView
+open LowStar.Modifies
+module M = LowStar.Modifies
+open LowStar.ModifiesPat
+open FStar.HyperStack.ST
+module HS = FStar.HyperStack
+open Interop
+open Types_s
+open AES_s
+open GCTR_s
+open GCM_s
+open GCM_helpers
+open GHash
+open X64.CPU_Features_s
+
+let pre_cond (h:HS.mem) (h_b:s8) (hash_b:s8) (input_b:s8) (num_bytes:UInt64.t) = 
+  live h h_b /\ live h hash_b /\ live h input_b /\  
+  disjoint h_b hash_b /\ 
+  disjoint h_b input_b /\ 
+  disjoint hash_b input_b /\ 
+  length h_b % 16 == 0 /\ length hash_b % 16 == 0 /\ length input_b % 16 == 0 /\
+  length input_b == 16 `op_Multiply` (bytes_to_quad_size (UInt64.v num_bytes)) /\
+  length h_b >= 16 /\
+  length hash_b >= 16 /\
+  pclmulqdq_enabled
+
+let buffer_to_quad (b:s8 { B.length b % 16 == 0 /\ B.length b > 0 }) (h:HS.mem) : GTot quad32 =
+  let b128 = BV.mk_buffer_view b Views.view128 in
+  BV.as_buffer_mk_buffer_view b Views.view128;
+  BV.get_view_mk_buffer_view b Views.view128;
+  BV.length_eq b128;
+  assert (B.length b >= 16);
+  assert (BV.length b128 > 0);
+  Seq.index (BV.as_seq h b128) 0
+
+let buffer_to_seq_quad (b:s8 { B.length b % 16 == 0 }) (h:HS.mem) : GTot (s:Seq.seq quad32 {Seq.length s == B.length b / 16} ) =
+  let b128 = BV.mk_buffer_view b Views.view128 in
+  BV.as_buffer_mk_buffer_view b Views.view128;
+  BV.get_view_mk_buffer_view b Views.view128;
+  BV.length_eq b128;
+  (BV.as_seq h b128)
+
+let post_cond (h:HS.mem) (h':HS.mem) (h_b:s8) (hash_b:s8) (input_b:s8) (num_bytes:UInt64.t) = 
+  live h h_b /\ live h hash_b /\ live h input_b /\ 
+  live h' h_b /\ live h' hash_b /\ live h' input_b /\
+  length h_b % 16 == 0 /\ length hash_b % 16 == 0 /\ length input_b % 16 == 0 /\
+  length input_b == 16 `op_Multiply` (bytes_to_quad_size (UInt64.v num_bytes)) /\
+  length h_b >= 16 /\
+  length hash_b >= 16 /\  
+  (let old_hash = buffer_to_quad hash_b h  in
+   let new_hash = buffer_to_quad hash_b h' in
+   let h_q      = buffer_to_quad h_b    h  in
+   let num_bytes = UInt64.v num_bytes in
+   (num_bytes == 0 ==> new_hash == old_hash) /\
+   (let input_bytes = Seq.slice (le_seq_quad32_to_bytes (buffer_to_seq_quad input_b h)) 0 num_bytes in
+    let padded_bytes = pad_to_128_bits input_bytes in
+    let input_quads = le_bytes_to_seq_quad32 padded_bytes in
+    num_bytes > 0 ==>
+      Seq.length input_quads > 0 /\
+      new_hash == ghash_incremental h_q old_hash input_quads
+   )
+   )  
+
+
+let full_post_cond (h:HS.mem) (h':HS.mem) (h_b:s8) (hash_b:s8) (input_b:s8) (num_bytes:UInt64.t)  =
+  post_cond h h' h_b hash_b input_b num_bytes  /\
+  M.modifies (M.loc_buffer hash_b) h h'
+
+val ghash_incremental_bytes_stdcall: h_b:s8 -> hash_b:s8 -> input_b:s8 -> num_bytes:UInt64.t -> Stack unit
+	(requires (fun h -> pre_cond h h_b hash_b input_b num_bytes ))
+	(ensures (fun h0 _ h1 -> full_post_cond h0 h1 h_b hash_b input_b num_bytes ))
