vale/code/arch/x64/interop/Gcm_load_xor_stdcall.fst
@@ -1,0 +1,228 @@
+module Gcm_load_xor_stdcall
+
+open LowStar.Buffer
+module B = LowStar.Buffer
+module BV = LowStar.BufferView
+open LowStar.Modifies
+module M = LowStar.Modifies
+open LowStar.ModifiesPat
+open FStar.HyperStack.ST
+module HS = FStar.HyperStack
+open Interop
+open Words_s
+open Types_s
+open X64.Machine_s
+open X64.Memory_s
+open X64.Vale.State
+open X64.Vale.Decls
+open BufferViewHelpers
+open Interop_assumptions
+open X64.Vale.StateLemmas
+open X64.Vale.Lemmas
+module TS = X64.Taint_Semantics_s
+module ME = X64.Memory_s
+module BS = X64.Bytes_Semantics_s
+
+friend SecretByte
+friend X64.Memory_s
+friend X64.Memory
+friend X64.Vale.Decls
+friend X64.Vale.StateLemmas
+#set-options "--z3rlimit 60"
+
+open Vale_gcm_load_xor_stdcall
+
+#set-options "--initial_fuel 6 --max_fuel 6 --initial_ifuel 0 --max_ifuel 0"
+let create_buffer_list (plain_b:s8) (mask_b:s8) (cipher_b:s8) (stack_b:b8)  : (l:list b8{
+    l == [stack_b;plain_b;mask_b;cipher_b] /\
+  (forall x. {:pattern List.memP x l} List.memP x l <==> (x == plain_b \/ x == mask_b \/ x == cipher_b \/ x == stack_b))}) =
+  [stack_b;plain_b;mask_b;cipher_b]
+
+#set-options "--max_fuel 0 --max_ifuel 0"
+
+let create_initial_trusted_state is_win plain_b mask_b cipher_b offset num_blocks key iv stack_b (h0:HS.mem{pre_cond h0 plain_b mask_b cipher_b (UInt64.uint_to_t offset) num_blocks key iv /\ B.length stack_b == 40 /\ live h0 stack_b /\ buf_disjoint_from stack_b [plain_b;mask_b;cipher_b]}) : GTot TS.traceState =
+  let taint_func (x:b8) : GTot taint =
+    if StrongExcludedMiddle.strong_excluded_middle (x == plain_b) then Secret else
+    if StrongExcludedMiddle.strong_excluded_middle (x == mask_b) then Secret else
+    if StrongExcludedMiddle.strong_excluded_middle (x == cipher_b) then Secret else
+    Public in
+  let buffers = create_buffer_list plain_b mask_b cipher_b stack_b in
+  let (mem:mem) = {addrs = addrs; ptrs = buffers; hs = h0} in
+  let addr_plain_b = addrs plain_b in
+  let addr_mask_b = addrs mask_b in
+  let addr_cipher_b = addrs cipher_b in
+  let addr_stack:nat64 = addrs stack_b + 0 in
+  let regs = if is_win then (
+    fun r -> begin match r with
+    | Rsp -> addr_stack
+    | Rcx -> addr_plain_b
+    | Rdx -> addr_mask_b
+    | R8 -> addr_cipher_b
+    | R9 -> offset
+    | _ -> init_regs r end)
+  else (
+    fun r -> begin match r with
+    | Rsp -> addr_stack
+    | Rdi -> addr_plain_b
+    | Rsi -> addr_mask_b
+    | Rdx -> addr_cipher_b
+    | Rcx -> offset
+    | _ -> init_regs r end)
+  in let regs = FunctionalExtensionality.on reg regs
+  in let xmms = FunctionalExtensionality.on xmm init_xmms in
+  let (s0:BS.state) = {BS.ok = true; BS.regs = regs; BS.xmms = xmms; BS.flags = 0;
+       BS.mem = Interop.down_mem h0 addrs buffers} in
+  {TS.state = s0; TS.trace = []; TS.memTaint = create_valid_memtaint mem buffers taint_func}
+
+val lemma_ghost_gcm_load_xor_stdcall: is_win:bool -> plain_b:s8 -> mask_b:s8 -> cipher_b:s8 -> offset:nat64 -> num_blocks:Ghost.erased (nat64) -> key:Ghost.erased (aes_key_LE AES_128) -> iv:Ghost.erased (quad32) ->  stack_b:b8 -> (h0:HS.mem{pre_cond h0 plain_b mask_b cipher_b (UInt64.uint_to_t offset) num_blocks key iv /\ B.length stack_b == 40 /\ live h0 stack_b /\ buf_disjoint_from stack_b [plain_b;mask_b;cipher_b]}) ->
+  Ghost (TS.traceState * nat * HS.mem)
+    (requires True)
+    (ensures (fun (s1, f1, h1) ->
+      (let s0 = create_initial_trusted_state is_win plain_b mask_b cipher_b offset num_blocks key iv stack_b h0 in
+      Some s1 == TS.taint_eval_code (va_code_gcm_load_xor_stdcall is_win) f1 s0 /\
+      Interop.correct_down h1 addrs [stack_b;plain_b;mask_b;cipher_b] s1.TS.state.BS.mem /\
+      post_cond h0 h1 plain_b mask_b cipher_b (UInt64.uint_to_t offset) num_blocks key iv  /\
+      calling_conventions is_win s0 s1 /\
+      M.modifies (M.loc_union (M.loc_buffer stack_b) ( M.loc_buffer cipher_b)) h0 h1)
+    ))
+
+// ===============================================================================================
+//  Everything below this line is untrusted
+
+let create_initial_vale_state is_win plain_b mask_b cipher_b offset num_blocks key iv stack_b (h0:HS.mem{pre_cond h0 plain_b mask_b cipher_b (UInt64.uint_to_t offset) num_blocks key iv /\ B.length stack_b == 40 /\ live h0 stack_b /\ buf_disjoint_from stack_b [plain_b;mask_b;cipher_b]}) : GTot va_state =
+  let taint_func (x:b8) : GTot taint =
+    if StrongExcludedMiddle.strong_excluded_middle (x == plain_b) then Secret else
+    if StrongExcludedMiddle.strong_excluded_middle (x == mask_b) then Secret else
+    if StrongExcludedMiddle.strong_excluded_middle (x == cipher_b) then Secret else
+    Public in
+  let buffers = create_buffer_list plain_b mask_b cipher_b stack_b in
+  let (mem:mem) = {addrs = addrs; ptrs = buffers; hs = h0} in
+  let addr_plain_b = addrs plain_b in
+  let addr_mask_b = addrs mask_b in
+  let addr_cipher_b = addrs cipher_b in
+  let addr_stack:nat64 = addrs stack_b + 0 in
+  let regs = if is_win then (
+    fun r -> begin match r with
+    | Rsp -> addr_stack
+    | Rcx -> addr_plain_b
+    | Rdx -> addr_mask_b
+    | R8 -> addr_cipher_b
+    | R9 -> offset
+    | _ -> init_regs r end)
+  else (
+    fun r -> begin match r with
+    | Rsp -> addr_stack
+    | Rdi -> addr_plain_b
+    | Rsi -> addr_mask_b
+    | Rdx -> addr_cipher_b
+    | Rcx -> offset
+    | _ -> init_regs r end)
+  in let regs = FunctionalExtensionality.on reg regs
+  in let xmms = FunctionalExtensionality.on xmm init_xmms in
+  {ok = true; regs = regs; xmms = xmms; flags = 0; mem = mem;
+      memTaint = create_valid_memtaint mem buffers taint_func}
+
+let create_lemma is_win plain_b mask_b cipher_b offset num_blocks key iv stack_b (h0:HS.mem{pre_cond h0 plain_b mask_b cipher_b (UInt64.uint_to_t offset) num_blocks key iv /\ B.length stack_b == 40 /\ live h0 stack_b /\ buf_disjoint_from stack_b [plain_b;mask_b;cipher_b]}) : Lemma
+  (create_initial_trusted_state is_win plain_b mask_b cipher_b offset num_blocks key iv stack_b h0 == state_to_S (create_initial_vale_state is_win plain_b mask_b cipher_b offset num_blocks key iv stack_b h0)) =
+    let s_init = create_initial_trusted_state is_win plain_b mask_b cipher_b offset num_blocks key iv stack_b h0 in
+    let s0 = create_initial_vale_state is_win plain_b mask_b cipher_b offset num_blocks key iv stack_b h0 in
+    let s1 = state_to_S s0 in
+    assert (FunctionalExtensionality.feq (regs' s1.TS.state) (regs' s_init.TS.state));
+    assert (FunctionalExtensionality.feq (xmms' s1.TS.state) (xmms' s_init.TS.state))
+
+let implies_pre (is_win:bool) (h0:HS.mem) (plain_b:s8) (mask_b:s8) (cipher_b:s8) (offset:nat64) (num_blocks:Ghost.erased (nat64)) (key:Ghost.erased (aes_key_LE AES_128)) (iv:Ghost.erased (quad32))  (stack_b:b8) : Lemma
+  (requires pre_cond h0 plain_b mask_b cipher_b (UInt64.uint_to_t offset) num_blocks key iv /\ B.length stack_b == 40 /\ live h0 stack_b /\ buf_disjoint_from stack_b [plain_b;mask_b;cipher_b])
+  (ensures (
+B.length stack_b == 40 /\ live h0 stack_b /\ buf_disjoint_from stack_b [plain_b;mask_b;cipher_b] /\ (
+  let s0 = create_initial_vale_state is_win plain_b mask_b cipher_b offset num_blocks key iv stack_b h0 in
+  length_t_eq (TBase TUInt64) stack_b;
+  length_t_eq (TBase TUInt128) plain_b;
+  length_t_eq (TBase TUInt128) mask_b;
+  length_t_eq (TBase TUInt128) cipher_b;
+  va_pre (va_code_gcm_load_xor_stdcall is_win) s0 is_win stack_b plain_b mask_b cipher_b offset (Ghost.reveal num_blocks) (Ghost.reveal key) (Ghost.reveal iv) ))) =
+  let va_s0 = create_initial_vale_state is_win plain_b mask_b cipher_b offset num_blocks key iv stack_b h0 in
+  assert (Seq.equal
+    (buffer128_as_seq (va_get_mem va_s0) plain_b)
+    (buffer_to_seq_quad32 plain_b va_s0.mem.hs));
+  assert (Seq.equal
+    (buffer128_as_seq (va_get_mem va_s0) cipher_b)
+    (buffer_to_seq_quad32 cipher_b va_s0.mem.hs));
+  let mask128 = BV.mk_buffer_view mask_b Views.view128 in
+  assert (Seq.equal (buffer_as_seq (va_get_mem va_s0) mask_b) (BV.as_seq va_s0.mem.hs mask128));
+  BV.as_seq_sel h0 mask128 0;   
+  length_t_eq (TBase TUInt64) stack_b;
+  length_t_eq (TBase TUInt128) plain_b;
+  length_t_eq (TBase TUInt128) mask_b;
+  length_t_eq (TBase TUInt128) cipher_b;
+  assert(Interop.disjoint stack_b plain_b);
+  assert(Interop.disjoint stack_b mask_b);
+  assert(Interop.disjoint stack_b cipher_b);
+  ()
+
+let implies_post (is_win:bool) (va_s0:va_state) (va_sM:va_state) (va_fM:va_fuel) (plain_b:s8) (mask_b:s8) (cipher_b:s8) (offset:nat64) (num_blocks:Ghost.erased (nat64)) (key:Ghost.erased (aes_key_LE AES_128)) (iv:Ghost.erased (quad32))  (stack_b:b8) : Lemma
+  (requires pre_cond va_s0.mem.hs plain_b mask_b cipher_b (UInt64.uint_to_t offset) num_blocks key iv /\ B.length stack_b == 40 /\ live va_s0.mem.hs stack_b /\ buf_disjoint_from stack_b [plain_b;mask_b;cipher_b]/\
+    va_post (va_code_gcm_load_xor_stdcall is_win) va_s0 va_sM va_fM is_win stack_b plain_b mask_b cipher_b offset (Ghost.reveal num_blocks) (Ghost.reveal key) (Ghost.reveal iv) )
+  (ensures post_cond va_s0.mem.hs va_sM.mem.hs plain_b mask_b cipher_b (UInt64.uint_to_t offset) num_blocks key iv ) =
+  length_t_eq (TBase TUInt64) stack_b;
+  length_t_eq (TBase TUInt128) plain_b;
+  length_t_eq (TBase TUInt128) mask_b;
+  length_t_eq (TBase TUInt128) cipher_b;
+  assert (Seq.equal
+    (buffer128_as_seq (va_get_mem va_s0) cipher_b)
+    (buffer_to_seq_quad32 cipher_b va_s0.mem.hs));
+  assert (Seq.equal
+    (buffer128_as_seq (va_get_mem va_sM) cipher_b)
+    (buffer_to_seq_quad32 cipher_b va_sM.mem.hs));
+  assert (Seq.equal
+    (buffer128_as_seq (va_get_mem va_sM) plain_b)
+    (buffer_to_seq_quad32 plain_b va_sM.mem.hs));
+  let mask128 = BV.mk_buffer_view mask_b Views.view128 in
+  assert (Seq.equal (buffer_as_seq (va_get_mem va_s0) mask_b) (BV.as_seq va_s0.mem.hs mask128));
+  BV.as_seq_sel va_s0.mem.hs mask128 0;  
+  ()
+
+#set-options "--max_fuel 0 --initial_ifuel 1 --max_ifuel 1"
+
+let lemma_ghost_gcm_load_xor_stdcall is_win plain_b mask_b cipher_b offset num_blocks key iv stack_b h0 =
+  length_t_eq (TBase TUInt64) stack_b;
+  length_t_eq (TBase TUInt128) plain_b;
+  length_t_eq (TBase TUInt128) mask_b;
+  length_t_eq (TBase TUInt128) cipher_b;
+  implies_pre is_win h0 plain_b mask_b cipher_b offset num_blocks key iv stack_b;
+  let s0 = create_initial_trusted_state is_win plain_b mask_b cipher_b offset num_blocks key iv stack_b h0 in
+  let s0' = create_initial_vale_state is_win plain_b mask_b cipher_b offset num_blocks key iv stack_b h0 in
+  create_lemma is_win plain_b mask_b cipher_b offset num_blocks key iv stack_b h0;
+  let s_v, f_v = va_lemma_gcm_load_xor_stdcall (va_code_gcm_load_xor_stdcall is_win) s0' is_win stack_b plain_b mask_b cipher_b offset (Ghost.reveal num_blocks) (Ghost.reveal key) (Ghost.reveal iv) in
+  implies_post is_win s0' s_v f_v plain_b mask_b cipher_b offset num_blocks key iv stack_b;
+  let s1 = Some?.v (TS.taint_eval_code (va_code_gcm_load_xor_stdcall is_win) f_v s0) in
+  assert (state_eq_S s1 (state_to_S s_v));
+  assert (FunctionalExtensionality.feq s1.TS.state.BS.regs s_v.regs);
+  assert (FunctionalExtensionality.feq s1.TS.state.BS.xmms s_v.xmms);
+  assert (M.modifies (M.loc_union (M.loc_buffer stack_b) ( M.loc_buffer cipher_b)) h0 s_v.mem.hs);
+  s1, f_v, s_v.mem.hs
+
+#set-options "--max_fuel 0 --max_ifuel 0"
+
+irreducible
+let gcm_load_xor_stdcall_aux (plain_b:s8) (mask_b:s8) (cipher_b:s8) (offset:UInt64.t) (num_blocks:Ghost.erased (nat64)) (key:Ghost.erased (aes_key_LE AES_128)) (iv:Ghost.erased (quad32)) (stack_b:b8) : Stack unit
+  (fun h -> pre_cond h plain_b mask_b cipher_b offset num_blocks key iv  /\ B.length stack_b == 40 /\ live h stack_b /\ buf_disjoint_from stack_b [plain_b;mask_b;cipher_b])
+  (fun h0 _ h1 ->
+    post_cond h0 h1 plain_b mask_b cipher_b offset num_blocks key iv  /\
+    M.modifies (M.loc_union (M.loc_buffer stack_b) ( M.loc_buffer cipher_b)) h0 h1) =
+  if win then
+  st_put
+    (fun h -> pre_cond h plain_b mask_b cipher_b offset num_blocks key iv /\ B.length stack_b == 40 /\ live h stack_b /\ buf_disjoint_from stack_b [plain_b;mask_b;cipher_b])
+    (fun h -> let _, _, h1 =
+      lemma_ghost_gcm_load_xor_stdcall true plain_b mask_b cipher_b (UInt64.v offset) num_blocks key iv stack_b h
+    in (), h1)
+  else st_put
+    (fun h -> pre_cond h plain_b mask_b cipher_b offset num_blocks key iv /\ B.length stack_b == 40 /\ live h stack_b /\ buf_disjoint_from stack_b [plain_b;mask_b;cipher_b])
+    (fun h -> let _, _, h1 =
+      lemma_ghost_gcm_load_xor_stdcall false plain_b mask_b cipher_b (UInt64.v offset) num_blocks key iv stack_b h
+    in (), h1)
+
+let gcm_load_xor_stdcall plain_b mask_b cipher_b offset num_blocks key iv  =
+  push_frame();
+  let (stack_b:b8) = B.alloca (UInt8.uint_to_t 0) (UInt32.uint_to_t 40) in
+  gcm_load_xor_stdcall_aux plain_b mask_b cipher_b offset num_blocks key iv stack_b;
+  pop_frame()
