vale/code/arch/x64/interop/Gcm_load_xor_stdcall.fsti
@@ -1,0 +1,84 @@
+module Gcm_load_xor_stdcall
+
+open LowStar.Buffer
+module B = LowStar.Buffer
+module BV = LowStar.BufferView
+open LowStar.Modifies
+module M = LowStar.Modifies
+open LowStar.ModifiesPat
+open FStar.HyperStack.ST
+module HS = FStar.HyperStack
+open Interop
+open Types_s
+open AES_s
+open GCTR_s
+open GCTR
+
+let buffer_to_quad32 (b:s8 { B.length b % 16 == 0 /\ B.length b > 0 }) (h:HS.mem) : GTot quad32 =
+  let b128 = BV.mk_buffer_view b Views.view128 in
+  BV.as_buffer_mk_buffer_view b Views.view128;
+  BV.get_view_mk_buffer_view b Views.view128;
+  BV.length_eq b128;
+  assert (B.length b >= 16);
+  assert (BV.length b128 > 0);
+  BV.sel h b128 0
+
+let buffer_to_seq_quad32 (b:s8{ B.length b % 16 == 0 }) (h:HS.mem) : GTot (s:Seq.seq quad32 {Seq.length s == B.length b / 16} ) =
+  let b128 = BV.mk_buffer_view b Views.view128 in
+  BV.as_buffer_mk_buffer_view b Views.view128;
+  BV.get_view_mk_buffer_view b Views.view128;
+  BV.length_eq b128;
+  (BV.as_seq h b128)
+
+let pre_cond (h:HS.mem) (plain_b:s8) (mask_b:s8) (cipher_b:s8) (offset:UInt64.t) (num_blocks:Ghost.erased (nat64)) (key:Ghost.erased (aes_key_LE AES_128)) (iv:Ghost.erased (quad32)) = 
+  live h plain_b /\ live h mask_b /\ live h cipher_b /\
+  disjoint plain_b mask_b /\ 
+  disjoint plain_b cipher_b /\ 
+  disjoint mask_b cipher_b /\ 
+  length plain_b % 16 == 0 /\ length mask_b % 16 == 0 /\ length cipher_b % 16 == 0 /\
+  (
+  length plain_b  >= (Ghost.reveal num_blocks) `op_Multiply` 16 /\
+  length cipher_b == length plain_b /\
+  length mask_b == 16 /\
+  (let offset = UInt64.v offset in
+   let num_blocks = (Ghost.reveal num_blocks) in
+   let mask   = buffer_to_quad32       mask_b h in
+   let plain  = buffer_to_seq_quad32  plain_b h in
+   let cipher = buffer_to_seq_quad32 cipher_b h in
+   let key = Ghost.reveal key in
+   let iv = Ghost.reveal iv in
+
+   // gcm_body specific
+   offset < num_blocks /\
+   mask == aes_encrypt_BE AES_128 key (inc32 iv offset) /\
+   gctr_partial AES_128 offset plain cipher key iv
+  )
+  )  
+
+let post_cond (h:HS.mem) (h':HS.mem) (plain_b:s8) (mask_b:s8) (cipher_b:s8) (offset:UInt64.t) (num_blocks:Ghost.erased (nat64)) (key:Ghost.erased (aes_key_LE AES_128)) (iv:Ghost.erased (quad32)) = 
+  live h plain_b /\ live h mask_b /\ live h cipher_b /\ 
+  live h' plain_b /\ live h' mask_b /\ live h' cipher_b /\ 
+  length plain_b % 16 == 0 /\ length mask_b % 16 == 0 /\ length cipher_b % 16 == 0 /\
+  length plain_b  >= (Ghost.reveal num_blocks) `op_Multiply` 16 /\
+  length cipher_b == length plain_b /\
+  length mask_b == 16 /\
+  (let offset = UInt64.v offset in
+   let num_blocks = (Ghost.reveal num_blocks) in
+   let mask   = buffer_to_quad32  mask_b h in
+   let plain  = buffer_to_seq_quad32  plain_b h' in
+   let old_cipher = buffer_to_seq_quad32 cipher_b h in
+   let cipher = buffer_to_seq_quad32 cipher_b h' in
+   let key = Ghost.reveal key in
+   let iv = Ghost.reveal iv in
+   offset < num_blocks /\
+   gctr_partial AES_128 (offset + 1) plain cipher key iv /\
+   Seq.slice cipher 0 offset == Seq.slice old_cipher 0 offset  // We didn't disrupt earlier slots
+  )  
+
+let full_post_cond (h:HS.mem) (h':HS.mem) (plain_b:s8) (mask_b:s8) (cipher_b:s8) (offset:UInt64.t) (num_blocks:Ghost.erased (nat64)) (key:Ghost.erased (aes_key_LE AES_128)) (iv:Ghost.erased (quad32))  =
+  post_cond h h' plain_b mask_b cipher_b offset num_blocks key iv  /\
+  M.modifies (M.loc_buffer cipher_b) h h'
+
+val gcm_load_xor_stdcall: plain_b:s8 -> mask_b:s8 -> cipher_b:s8 -> offset:UInt64.t -> num_blocks:Ghost.erased (nat64) -> key:Ghost.erased (aes_key_LE AES_128) -> iv:Ghost.erased (quad32) -> Stack unit
+	(requires (fun h -> pre_cond h plain_b mask_b cipher_b offset num_blocks key iv ))
+	(ensures (fun h0 _ h1 -> full_post_cond h0 h1 plain_b mask_b cipher_b offset num_blocks key iv ))
