vale/code/arch/x64/interop/Gctr_extra_stdcall.fsti
@@ -1,0 +1,112 @@
+module Gctr_extra_stdcall
+
+open LowStar.Buffer
+module B = LowStar.Buffer
+module BV = LowStar.BufferView
+open LowStar.Modifies
+module M = LowStar.Modifies
+open LowStar.ModifiesPat
+open FStar.HyperStack.ST
+module HS = FStar.HyperStack
+open Interop
+open Types_s
+open Words_s
+open AES_s
+open GCTR_s
+open GCTR
+open GCM_s
+open GCM_helpers
+open GHash
+
+let buffer_to_seq_quad32 (b:s8{ B.length b % 16 == 0 }) (h:HS.mem) : GTot (s:Seq.seq quad32 {Seq.length s == B.length b / 16} ) =
+  let b128 = BV.mk_buffer_view b Views.view128 in
+  BV.as_buffer_mk_buffer_view b Views.view128;
+  BV.get_view_mk_buffer_view b Views.view128;
+  BV.length_eq b128;
+  (BV.as_seq h b128)
+
+let buffer_to_quad32 (b:s8 { B.length b % 16 == 0 /\ B.length b > 0 }) (h:HS.mem) : GTot quad32 =
+  let b128 = BV.mk_buffer_view b Views.view128 in
+  BV.as_buffer_mk_buffer_view b Views.view128;
+  BV.get_view_mk_buffer_view b Views.view128;
+  BV.length_eq b128;
+  assert (B.length b >= 16);
+  assert (BV.length b128 > 0);
+  BV.sel h b128 0
+
+let keys_match (key:Ghost.erased (aes_key_LE AES_128)) (keys_b:s8 { B.length keys_b % 16 == 0 }) (h:HS.mem) =
+  let keys128_b = BV.mk_buffer_view keys_b Views.view128 in
+  let round_keys = key_to_round_keys_LE AES_128 (Ghost.reveal key) in
+  BV.as_seq h keys128_b == round_keys
+
+let pre_cond (h:HS.mem) (plain_b:s8) (num_bytes:nat64) (iv_old:Ghost.erased (quad32)) (iv_b:s8) (key:Ghost.erased (aes_key_LE AES_128)) (keys_b:s8) (cipher_b:s8) = 
+  live h plain_b /\ live h iv_b /\ live h keys_b /\ live h cipher_b /\ 
+  disjoint plain_b iv_b /\ 
+  disjoint plain_b keys_b /\ 
+  disjoint plain_b cipher_b /\ 
+  disjoint iv_b keys_b /\ 
+  disjoint iv_b cipher_b /\ 
+  disjoint keys_b cipher_b /\ 
+length plain_b % 16 == 0 /\ length iv_b % 16 == 0 /\ length keys_b % 16 == 0 /\ length cipher_b % 16 == 0 /\
+
+  length plain_b == bytes_to_quad_size num_bytes `op_Multiply` 16 /\
+  length cipher_b == length plain_b /\
+  length iv_b == 16 /\
+
+  4096 `op_Multiply` num_bytes < pow2_32 /\
+  256 `op_Multiply` bytes_to_quad_size num_bytes < pow2_32 /\
+
+  // AES reqs
+  length keys_b == (nr AES_128 + 1) `op_Multiply` 16 /\
+  length keys_b % 16 == 0 /\  // REVIEW: Should be derivable from line above :(
+  keys_match key keys_b h /\
+
+  // Extra reqs
+  (let num_bytes = num_bytes in
+   let num_blocks = num_bytes / 16 in
+   let iv = buffer_to_quad32 iv_b h in
+   num_bytes % 16 <> 0 /\
+   0 < num_bytes /\ num_bytes < 16 `op_Multiply` bytes_to_quad_size num_bytes /\
+   16 `op_Multiply` (bytes_to_quad_size num_bytes - 1) < num_bytes /\
+   gctr_partial AES_128
+                num_blocks
+                (buffer_to_seq_quad32 plain_b h)
+                (buffer_to_seq_quad32  cipher_b h)
+                (Ghost.reveal key)
+                (Ghost.reveal iv_old) /\
+   iv == inc32 (Ghost.reveal iv_old) num_blocks)
+   
+
+let post_cond (h:HS.mem) (h':HS.mem) (plain_b:s8) (num_bytes:nat64) (iv_old:Ghost.erased (quad32)) (iv_b:s8) (key:Ghost.erased (aes_key_LE AES_128)) (keys_b:s8) (cipher_b:s8) = 
+  live h plain_b /\ live h iv_b /\ live h keys_b /\ live h cipher_b /\ 
+  live h' plain_b /\ live h' iv_b /\ live h' keys_b /\ live h' cipher_b /\ 
+  length plain_b % 16 == 0 /\ length iv_b % 16 == 0 /\ length keys_b % 16 == 0 /\ length cipher_b % 16 == 0 /\
+
+  length plain_b  == bytes_to_quad_size num_bytes `op_Multiply` 16 /\
+  length cipher_b == length plain_b /\
+  length iv_b == 16 /\
+  length plain_b % 16 == 0 /\
+  length keys_b == (nr AES_128 + 1) `op_Multiply` 16 /\
+
+  (let num_bytes = num_bytes in
+   let num_blocks = num_bytes / 16 in
+   let iv_new = buffer_to_quad32 iv_b h in
+
+   // We modified cipher_b, but we didn't disrupt the work that was previously done
+   let cipher_blocks  = Seq.slice (buffer_to_seq_quad32 cipher_b h)  0 num_blocks in
+   let cipher_blocks' = Seq.slice (buffer_to_seq_quad32 cipher_b h') 0 num_blocks in
+   cipher_blocks == cipher_blocks' /\
+
+   // GCTR
+   (let plain  = Seq.slice (le_seq_quad32_to_bytes (buffer_to_seq_quad32  plain_b h))  0 num_bytes in
+    let cipher = Seq.slice (le_seq_quad32_to_bytes (buffer_to_seq_quad32 cipher_b h')) 0 num_bytes in
+    cipher == gctr_encrypt_LE (Ghost.reveal iv_old) (make_gctr_plain_LE plain) AES_128 (Ghost.reveal key))
+    )
+  
+let full_post_cond (h:HS.mem) (h':HS.mem) (plain_b:s8) (num_bytes:nat64) (iv_old:Ghost.erased (quad32)) (iv_b:s8) (key:Ghost.erased (aes_key_LE AES_128)) (keys_b:s8) (cipher_b:s8)  =
+  post_cond h h' plain_b num_bytes iv_old iv_b key keys_b cipher_b  /\
+  M.modifies (M.loc_buffer cipher_b) h h'
+
+val gctr_bytes_extra_stdcall: plain_b:s8 -> num_bytes:nat64 -> iv_old:Ghost.erased (quad32) -> iv_b:s8 -> key:Ghost.erased (aes_key_LE AES_128) -> keys_b:s8 -> cipher_b:s8 -> Stack unit
+	(requires (fun h -> pre_cond h plain_b num_bytes iv_old iv_b key keys_b cipher_b ))
+	(ensures (fun h0 _ h1 -> full_post_cond h0 h1 plain_b num_bytes iv_old iv_b key keys_b cipher_b ))
