vale/code/arch/x64/interop/Vale_quad32_xor_stdcall.fst
@@ -1,0 +1,24 @@
+module Vale_quad32_xor_stdcall
+
+open X64.Machine_s
+open X64.Memory
+open X64.Vale.State
+open X64.Vale.Decls
+open X64.Util
+
+val va_code_quad32_xor_stdcall: bool -> va_code
+
+let va_code_quad32_xor_stdcall = va_code_quad32_xor_stdcall
+
+let va_pre (va_b0:va_code) (va_s0:va_state) (win:bool) (stack_b:buffer64)
+(src1:buffer128) (src2:buffer128) (dst:buffer128)  = va_req_quad32_xor_stdcall va_b0 va_s0 win stack_b src1 src2 dst 
+
+let va_post (va_b0:va_code) (va_s0:va_state) (va_sM:va_state) (va_fM:va_fuel) (win:bool)  (stack_b:buffer64)
+(src1:buffer128) (src2:buffer128) (dst:buffer128)  = va_ens_quad32_xor_stdcall va_b0 va_s0 win stack_b src1 src2 dst va_sM va_fM
+
+val va_lemma_quad32_xor_stdcall(va_b0:va_code) (va_s0:va_state) (win:bool) (stack_b:buffer64)
+(src1:buffer128) (src2:buffer128) (dst:buffer128) : Ghost ((va_sM:va_state) * (va_fM:va_fuel))
+  (requires va_pre va_b0 va_s0 win stack_b src1 src2 dst )
+  (ensures (fun (va_sM, va_fM) -> va_post va_b0 va_s0 va_sM va_fM win stack_b src1 src2 dst ))
+
+let va_lemma_quad32_xor_stdcall = va_lemma_quad32_xor_stdcall
