vale/code/arch/x64/interop/Zero_quad32_stdcall.fst
@@ -1,0 +1,179 @@
+module Zero_quad32_stdcall
+
+open LowStar.Buffer
+module B = LowStar.Buffer
+module BV = LowStar.BufferView
+open LowStar.Modifies
+module M = LowStar.Modifies
+open LowStar.ModifiesPat
+open FStar.HyperStack.ST
+module HS = FStar.HyperStack
+open Interop
+open Words_s
+open Types_s
+open X64.Machine_s
+open X64.Memory_s
+open X64.Vale.State
+open X64.Vale.Decls
+open BufferViewHelpers
+open Interop_assumptions
+open X64.Vale.StateLemmas
+open X64.Vale.Lemmas
+module TS = X64.Taint_Semantics_s
+module ME = X64.Memory_s
+module BS = X64.Bytes_Semantics_s
+
+friend SecretByte
+friend X64.Memory_s
+friend X64.Memory
+friend X64.Vale.Decls
+friend X64.Vale.StateLemmas
+#set-options "--z3rlimit 60"
+
+open Vale_zero_quad32_stdcall
+
+#set-options "--initial_fuel 4 --max_fuel 4 --initial_ifuel 0 --max_ifuel 0"
+let create_buffer_list (b:s8) (stack_b:b8)  : (l:list b8{
+    l == [stack_b;b] /\
+  (forall x. {:pattern List.memP x l} List.memP x l <==> (x == b \/ x == stack_b))}) =
+  [stack_b;b]
+
+#set-options "--max_fuel 0 --max_ifuel 0"
+
+let create_initial_trusted_state is_win b stack_b (h0:HS.mem{pre_cond h0 b /\ B.length stack_b == 16 /\ live h0 stack_b /\ buf_disjoint_from stack_b [b]}) : GTot TS.traceState =
+  let taint_func (x:b8) : GTot taint =
+    if StrongExcludedMiddle.strong_excluded_middle (x == b) then Secret else
+    Public in
+  let buffers = create_buffer_list b stack_b in
+  let (mem:mem) = {addrs = addrs; ptrs = buffers; hs = h0} in
+  let addr_b = addrs b in
+  let addr_stack:nat64 = addrs stack_b + 0 in
+  let regs = if is_win then (
+    fun r -> begin match r with
+    | Rsp -> addr_stack
+    | Rcx -> addr_b
+    | _ -> init_regs r end)
+  else (
+    fun r -> begin match r with
+    | Rsp -> addr_stack
+    | Rdi -> addr_b
+    | _ -> init_regs r end)
+  in let regs = FunctionalExtensionality.on reg regs
+  in let xmms = FunctionalExtensionality.on xmm init_xmms in
+  let (s0:BS.state) = {BS.ok = true; BS.regs = regs; BS.xmms = xmms; BS.flags = 0;
+       BS.mem = Interop.down_mem h0 addrs buffers} in
+  {TS.state = s0; TS.trace = []; TS.memTaint = create_valid_memtaint mem buffers taint_func}
+
+val lemma_ghost_zero_quad32_stdcall: is_win:bool -> b:s8 ->  stack_b:b8 -> (h0:HS.mem{pre_cond h0 b /\ B.length stack_b == 16 /\ live h0 stack_b /\ buf_disjoint_from stack_b [b]}) ->
+  Ghost (TS.traceState * nat * HS.mem)
+    (requires True)
+    (ensures (fun (s1, f1, h1) ->
+      (let s0 = create_initial_trusted_state is_win b stack_b h0 in
+      Some s1 == TS.taint_eval_code (va_code_zero_quad32_stdcall is_win) f1 s0 /\
+      Interop.correct_down h1 addrs [stack_b;b] s1.TS.state.BS.mem /\
+      post_cond h0 h1 b  /\
+      calling_conventions is_win s0 s1 /\
+      M.modifies (M.loc_union (M.loc_buffer stack_b) ( M.loc_buffer b)) h0 h1)
+    ))
+
+// ===============================================================================================
+//  Everything below this line is untrusted
+
+let create_initial_vale_state is_win b stack_b (h0:HS.mem{pre_cond h0 b /\ B.length stack_b == 16 /\ live h0 stack_b /\ buf_disjoint_from stack_b [b]}) : GTot va_state =
+  let taint_func (x:b8) : GTot taint =
+    if StrongExcludedMiddle.strong_excluded_middle (x == b) then Secret else
+    Public in
+  let buffers = create_buffer_list b stack_b in
+  let (mem:mem) = {addrs = addrs; ptrs = buffers; hs = h0} in
+  let addr_b = addrs b in
+  let addr_stack:nat64 = addrs stack_b + 0 in
+  let regs = if is_win then (
+    fun r -> begin match r with
+    | Rsp -> addr_stack
+    | Rcx -> addr_b
+    | _ -> init_regs r end)
+  else (
+    fun r -> begin match r with
+    | Rsp -> addr_stack
+    | Rdi -> addr_b
+    | _ -> init_regs r end)
+  in let regs = FunctionalExtensionality.on reg regs
+  in let xmms = FunctionalExtensionality.on xmm init_xmms in
+  {ok = true; regs = regs; xmms = xmms; flags = 0; mem = mem;
+      memTaint = create_valid_memtaint mem buffers taint_func}
+
+let create_lemma is_win b stack_b (h0:HS.mem{pre_cond h0 b /\ B.length stack_b == 16 /\ live h0 stack_b /\ buf_disjoint_from stack_b [b]}) : Lemma
+  (create_initial_trusted_state is_win b stack_b h0 == state_to_S (create_initial_vale_state is_win b stack_b h0)) =
+    let s_init = create_initial_trusted_state is_win b stack_b h0 in
+    let s0 = create_initial_vale_state is_win b stack_b h0 in
+    let s1 = state_to_S s0 in
+    assert (FunctionalExtensionality.feq (regs' s1.TS.state) (regs' s_init.TS.state));
+    assert (FunctionalExtensionality.feq (xmms' s1.TS.state) (xmms' s_init.TS.state))
+
+let implies_pre (is_win:bool) (h0:HS.mem) (b:s8)  (stack_b:b8) : Lemma
+  (requires pre_cond h0 b /\ B.length stack_b == 16 /\ live h0 stack_b /\ buf_disjoint_from stack_b [b])
+  (ensures (
+B.length stack_b == 16 /\ live h0 stack_b /\ buf_disjoint_from stack_b [b] /\ (
+  let s0 = create_initial_vale_state is_win b stack_b h0 in
+  length_t_eq (TBase TUInt64) stack_b;
+  length_t_eq (TBase TUInt128) b;
+  va_pre (va_code_zero_quad32_stdcall is_win) s0 is_win stack_b b ))) =
+  length_t_eq (TBase TUInt64) stack_b;
+  length_t_eq (TBase TUInt128) b;
+  assert(Interop.disjoint stack_b b);
+  ()
+
+let implies_post (is_win:bool) (va_s0:va_state) (va_sM:va_state) (va_fM:va_fuel) (b:s8)  (stack_b:b8) : Lemma
+  (requires pre_cond va_s0.mem.hs b /\ B.length stack_b == 16 /\ live va_s0.mem.hs stack_b /\ buf_disjoint_from stack_b [b]/\
+    va_post (va_code_zero_quad32_stdcall is_win) va_s0 va_sM va_fM is_win stack_b b )
+  (ensures post_cond va_s0.mem.hs va_sM.mem.hs b ) =
+  length_t_eq (TBase TUInt64) stack_b;
+  length_t_eq (TBase TUInt128) b;
+  let b128 = BV.mk_buffer_view b Views.view128 in
+  assert (Seq.equal (buffer_as_seq (va_get_mem va_sM) b) (BV.as_seq va_sM.mem.hs b128));
+  BV.as_seq_sel va_sM.mem.hs b128 0;  
+  ()
+
+#set-options "--max_fuel 0 --initial_ifuel 1 --max_ifuel 1"
+
+let lemma_ghost_zero_quad32_stdcall is_win b stack_b h0 =
+  length_t_eq (TBase TUInt64) stack_b;
+  length_t_eq (TBase TUInt128) b;
+  implies_pre is_win h0 b stack_b;
+  let s0 = create_initial_trusted_state is_win b stack_b h0 in
+  let s0' = create_initial_vale_state is_win b stack_b h0 in
+  create_lemma is_win b stack_b h0;
+  let s_v, f_v = va_lemma_zero_quad32_stdcall (va_code_zero_quad32_stdcall is_win) s0' is_win stack_b b in
+  implies_post is_win s0' s_v f_v b stack_b;
+  let s1 = Some?.v (TS.taint_eval_code (va_code_zero_quad32_stdcall is_win) f_v s0) in
+  assert (state_eq_S s1 (state_to_S s_v));
+  assert (FunctionalExtensionality.feq s1.TS.state.BS.regs s_v.regs);
+  assert (FunctionalExtensionality.feq s1.TS.state.BS.xmms s_v.xmms);
+  assert (M.modifies (M.loc_union (M.loc_buffer stack_b) ( M.loc_buffer b)) h0 s_v.mem.hs);
+  s1, f_v, s_v.mem.hs
+
+#set-options "--max_fuel 0 --max_ifuel 0"
+
+irreducible
+let zero_quad32_stdcall_aux (b:s8) (stack_b:b8) : Stack unit
+  (fun h -> pre_cond h b  /\ B.length stack_b == 16 /\ live h stack_b /\ buf_disjoint_from stack_b [b])
+  (fun h0 _ h1 ->
+    post_cond h0 h1 b  /\
+    M.modifies (M.loc_union (M.loc_buffer stack_b) ( M.loc_buffer b)) h0 h1) =
+  if win then
+  st_put
+    (fun h -> pre_cond h b /\ B.length stack_b == 16 /\ live h stack_b /\ buf_disjoint_from stack_b [b])
+    (fun h -> let _, _, h1 =
+      lemma_ghost_zero_quad32_stdcall true b stack_b h
+    in (), h1)
+  else st_put
+    (fun h -> pre_cond h b /\ B.length stack_b == 16 /\ live h stack_b /\ buf_disjoint_from stack_b [b])
+    (fun h -> let _, _, h1 =
+      lemma_ghost_zero_quad32_stdcall false b stack_b h
+    in (), h1)
+
+let zero_quad32_stdcall b  =
+  push_frame();
+  let (stack_b:b8) = B.alloca (UInt8.uint_to_t 0) (UInt32.uint_to_t 16) in
+  zero_quad32_stdcall_aux b stack_b;
+  pop_frame()
